---
layout: post
title:  "Mathematics Magazine, Vol. 79, December 2006"
subtitle: "Proposed by M. Goldenberg and M. Kaplan, USA."
date:   2015-11-17 16:16:01 -0600
categories: problem-solving
imgpath: "/assets/post/controllo-del-pendolo/img"
---

Let $F_n$ be the $n$th Fibonacci number, that is, $F_0=0$, $F_1=1$, and $F_n=F_{n-1}+F_{n-2}$ for $n\geq 2$. Prove that


$$\prod_{n=2}^{\infty}{F_{2n}+1\over F_{2n}-1}=3.$$


<em>Solution proposed by G.R.A.20 Problem Solving Group, Roma, Italy.</em>

<br><br>
First we note that for $N\geq 2$

$$S_N:=\log \left(\prod_{n=2}^{N}{F_{2n}+1\over F_{2n}-1}\right)=2\sum_{n=2}^{N}\mbox{arctanh}(1/F_{2n})$$

where


$$\mbox{arctanh}(x)={1\over 2}\log\left({1+x\over 1-x}\right) \quad \mbox{for $|x|\lt1$}.$$

We have to show that $\lim_{N\to \infty}S_N=\log 3$. Since

$$
\begin{eqnarray*}
\mbox{arctanh}(x)-\mbox{arctanh}(y)&=&{1\over 2}\log\left({(1+x)(1-y)\over (1-x)(1+y)}\right)\\
&=&{1\over 2}\log\left({(1-xy)+(x-y)\over (1-xy)-(x-y)}\right)=\mbox{arctanh}\left({x-y\over 1-xy}\right)
\end{eqnarray*}
$$


then

$$\mbox{arctanh}(1/F_{2n-1})-\mbox{arctanh}(1/F_{2n+1})=
\mbox{arctanh}\left({F_{2n+1}-F_{2n-1}\over F_{2n+1}F_{2n-1}-1}\right)=\mbox{arctanh}(1/F_{2n})$$

because $F_{2n+1}-F_{2n-1}=F_{2n}$ and $F_{2n+1}F_{2n-1}-1=F_{2n}^2$.
Therefore

$$S_N=2\sum_{n=2}^{N}\left(\mbox{arctanh}(1/F_{2n-1})-\mbox{arctanh}(1/F_{2n+1})\right)=2\left(\mbox{arctanh}(1/F_{3})-\mbox{arctanh}(1/F_{2N+1})\right)$$
and finally

$$\lim_{N\to \infty}S_N=2\,\mbox{arctanh}(1/F_{3})=2\,\mbox{arctanh}(1/2)=\log 3.$$

$$\square$$
